reorganize

Iterator/Combinators.lean
@@ -5,6 +5,7 @@ Authors: Paul Reichert
 -/
 prelude
 import Iterator.Wrapper
+import Iterator.AbstractIteration
 
 section FilterMap
 
@@ -73,92 +74,6 @@ section FlatMap
 -- todo: more universe polymorphism
 variable {m : Type u → Type u} {α α' β β' : Type u} [Iterator α m β] [Iterator α' m β'] {f : β → α'}
 
-abbrev RawStep (α β) := IterStep α β (fun _ _ => True) (fun _ => True) True
-
-abbrev IterStep.for {α β m} [Iterator α m β] (it : α) := IterStep α β (Iterator.yielded it) (Iterator.skipped it) (Iterator.finished it)
-
-structure Iteration (m) [Monad m] (γ : Type u) where
-  prop : γ → Prop
-  elem : m { c // prop c }
-
-@[inline]
-def Iteration.pure {γ m} [Monad m] (c : γ) : Iteration m γ :=
-  { prop c' := (c' = c), elem := Pure.pure ⟨c, rfl⟩ }
-
-@[inline]
-def Iteration.bind {γ δ m} [Monad m] (t : Iteration m γ) (f : γ → Iteration m δ) : Iteration m δ :=
-  { prop d := ∃ c, (f c).prop d ∧ t.prop c, elem :=
-    Bind.bind t.elem (fun c => (fun x => ⟨x.1, ⟨c.1, x.2, c.2⟩⟩) <$> (f c.1).elem) }
-
-#print Iteration.bind
-
-instance (m) [Monad m] : Monad (Iteration m) where
-  pure := Iteration.pure
-  bind := Iteration.bind
-
-@[inline]
-def Iteration.step {α β : Type u} [Iterator α m β] [Monad m] (it : α) : Iteration m (IterStep.for it) :=
-  { prop
-      | .yield it' b _ => Iterator.yielded it it' b
-      | .skip it' _ => Iterator.skipped it it'
-      | .done _ => Iterator.finished it,
-    elem := (fun step => ⟨step, match step with
-        | .yield _ _ h => h
-        | .skip _ h => h
-        | .done h => h⟩) <$> Iterator.step it
-  }
-
-@[inline]
-def Iteration.instIterator [Monad m] (stepFn : α → Iteration m (RawStep α β)) : Iterator α m β where
-  yielded it it' b := (stepFn it).prop (.yield it' b ⟨⟩)
-  skipped it it' := (stepFn it).prop (.skip it' ⟨⟩)
-  finished it := (stepFn it).prop (.done ⟨⟩)
-  step it := (match · with
-    | ⟨.yield it' b _, h⟩ => .yield it' b h
-    | ⟨.skip it' _, h⟩ => .skip it' h
-    | ⟨.done _, h⟩ => .done h) <$> (stepFn it).elem
-
-/-
-Ideas: use transitivity of the relation, flatMapStepSome
-
-Can I introduce a kind of generator monad?
-
-do
-  yield 1
-  yield 2
-  lift <| println "hi"
-  for x in l do
-    yield x
-
-it.bind (fun x => it₂ x)
-
-Iterators with a return type!
--/
-
--- instance [Functor m] [Iterator α m β] [Iterator α' m β'] : Iterator (FlatMapAux α f) m β' where
---   yielded it it' b := FlatMap.rawStep_eq it (.yield it' b ⟨⟩)
---     -- | { it₁, it₂ := some it₂ }, { it₁ := it₁', it₂ := some it₂' }, b => it₁ = it₁' ∧ Iterator.yielded it₂ it₂' b
---     -- | _, _, _ => False
---   skipped it it' := FlatMap.rawStep_eq it (.skip it' ⟨⟩)
---     -- | { it₁, it₂ := none }, { it₁ := it₁', it₂ := none } => Iterator.skipped it₁ it₁'
---     -- | { it₁, it₂ := none }, { it₁ := it₁', it₂ := some it₂' } => ∃ b, f b = it₂' ∧ Iterator.yielded it₁ it₁' b
---     -- | { it₁, it₂ := some it₂ }, { it₁ := it₁', it₂ := none } => it₁ = it₁' ∧ Iterator.finished it₂
---     -- | { it₁, it₂ := some it₂ }, { it₁ := it₁', it₂ := some it₂' } => it₁ = it₁' ∧ Iterator.skipped it₂ it₂'
---   finished it := FlatMap.rawStep_eq it (.done ⟨⟩)
---     -- | { it₁, it₂ := none } => Iterator.finished it₁
---     -- | _ => False
---   step
---     | { it₁, it₂ := none } =>
---       (match · with
---       | .yield it₁' b h => .skip { it₁ := it₁', it₂ := some (f b) } (.inl ⟨it₁', b, h, rfl⟩)
---       | .skip it₁' h => .skip { it₁ := it₁', it₂ := none } (.inr <| .inl ⟨it₁', h, rfl⟩)
---       | .done h => .done (.inr <| .inr ⟨h, rfl⟩)) <$> Iterator.step it₁
---     | { it₁, it₂ := some it₂ } =>
---       (match · with
---         | .yield it₂' b h => .yield { it₁ := it₁, it₂ := some it₂' } b (.inl ⟨it₂', b, h, rfl⟩)
---         | .skip it₂' h => .skip { it₁ := it₁, it₂ := some it₂' } (.inr <| .inl ⟨it₂', h, rfl⟩)
---         | .done h => .skip { it₁ := it₁, it₂ := none } (.inr <| .inr ⟨h, rfl⟩)) <$> Iterator.step it₂
-
 structure FlatMap (α) (f : β → α') where
   it₁ : α
   it₂ : Option α'
@@ -166,43 +81,6 @@ structure FlatMap (α) (f : β → α') where
 @[inline]
 def FlatMap.init (it : α) (f : β → α') : FlatMap α f :=
   ⟨it, none⟩
-
-@[inline]
-def matchStep [Monad m] [Iterator α m β] (it : α)
-    (yield : α → β → Iteration m γ) (skip : α → Iteration m γ) (done : Iteration m γ) := do
-  match ← Iteration.step it with
-  | .yield it' b _ => yield it' b
-  | .skip it' _ => skip it'
-  | .done _ => done
-
-theorem finite_instIterator {α} [Monad m] (stepFn : α → Iteration m (RawStep α β)) {rel : α → α → Prop} (hwf : WellFounded rel) :
-    letI : Iterator α m β := Iteration.instIterator stepFn
-    (h : ∀ it it', (IterStep.successor <$> stepFn it).prop (some it') → rel it' it) → Finite α := by
-  letI : Iterator α m β := Iteration.instIterator stepFn
-  intro h
-  refine ⟨?_⟩
-  refine Subrelation.wf ?_ <| InvImage.wf FiniteIteratorWF.inner hwf
-  intro it it' hlt
-  specialize h it'.inner it.inner
-  apply h
-  simp [Functor.map, Iteration.bind, Iteration.pure]
-  simp [FiniteIteratorWF.lt, Iteration.instIterator] at hlt
-  obtain ⟨b, hlt⟩ | hlt := hlt
-  · exact ⟨_, rfl, hlt⟩
-  · exact ⟨_, rfl, hlt⟩
-
-theorem productive_instIterator {α} [Monad m] (stepFn : α → Iteration m (RawStep α β)) {rel : α → α → Prop} (hwf : WellFounded rel) :
-    letI : Iterator α m β := Iteration.instIterator stepFn
-    (h : ∀ it it', (stepFn it).prop (.skip it' ⟨⟩) → rel it' it) → Productive α := by
-  letI : Iterator α m β := Iteration.instIterator stepFn
-  intro h
-  refine ⟨?_⟩
-  refine Subrelation.wf ?_ <| InvImage.wf ProductiveIteratorWF.inner hwf
-  intro it it' hlt
-  specialize h it'.inner it.inner
-  apply h
-  simp [ProductiveIteratorWF.lt, Iteration.instIterator] at hlt
-  exact hlt
 
 @[inline]
 def flatMapStepNone [Monad m] [Iterator α m β] [Iterator α' m β'] (f : β → α') (it₁ : α) :
@@ -236,71 +114,8 @@ theorem FlatMap.lex_of_right {f : β → α'} {r₁ : α → α → Prop} {r₂ 
     (h : r₂ it₂' it₂) : FlatMap.lex f r₁ r₂ ⟨it₁, it₂'⟩ ⟨it₁, it₂⟩ :=
   Prod.Lex.right _ h
 
-theorem Iteration.prop_bind {α β m} [Monad m] (f : α → Iteration m β) (t : Iteration m α) (b : β) :
-    (t >>= f).prop b ↔ ∃ a, (f a).prop b ∧ t.prop a :=
-  Iff.rfl
-
-theorem Iteration.prop_map {α β m} [Monad m] (f : α → β) (t : Iteration m α) (b : β) :
-    (f <$> t).prop b ↔ ∃ a, b = f a ∧ t.prop a :=
-  Iff.rfl
-
-theorem prop_successor_matchStep {α β γ : Type u} {m} [Monad m] [Iterator α m β] {it : α} {yield skip done}
-    {f : γ → δ} {x : δ}
-    (h : (f <$> matchStep (γ := γ) it yield skip done).prop x) :
-    (∃ it' b, Iterator.yielded it it' b ∧ (f <$> yield it' b).prop x) ∨
-    (∃ it', Iterator.skipped it it' ∧ (f <$> skip it').prop x) ∨
-    (Iterator.finished it ∧ (f <$> done).prop x) := by
-  simp only [Iteration.prop_map, matchStep, Iteration.prop_bind] at h
-  obtain ⟨c, rfl, _, h, h'⟩ := h
-  split at h
-  · exact Or.inl ⟨_, _, ‹_›, ⟨c, rfl, h⟩⟩
-  · exact Or.inr <| Or.inl ⟨_, ‹_›, ⟨c, rfl, h⟩⟩
-  · exact Or.inr <| Or.inr ⟨‹_›, ⟨c, rfl, h⟩⟩
-
-theorem FiniteIteratorWF.lt_iff_successor {α β : Type u} {m} [Monad m] [Iterator α m β] {it it' : FiniteIteratorWF α} :
-    it'.lt it ↔ (IterStep.successor <$> Iteration.step it.inner).prop (some it'.inner) := by
-  simp only [FiniteIteratorWF.lt, Functor.map, Iteration.bind, Iteration.pure, Function.comp_apply,
-    Iteration.step]
-  apply Iff.intro
-  · intro h
-    obtain ⟨b, h⟩ | h := h
-    · refine ⟨.yield it'.inner b h, rfl, h⟩
-    · refine ⟨.skip it'.inner h, rfl, h⟩
-  · intro h
-    obtain ⟨c, h, h'⟩ := h
-    split at h'
-    · simp only [IterStep.successor, Option.some.injEq] at h
-      exact h ▸ Or.inl ⟨_, h'⟩
-    · simp only [IterStep.successor, Option.some.injEq] at h
-      exact h ▸ Or.inr h'
-    · simp only [IterStep.successor, reduceCtorEq] at h
-
 def rel [Iterator α m β] [Iterator α' m β'] : FlatMap α f → FlatMap α f → Prop :=
   FlatMap.lex f (InvImage FiniteIteratorWF.lt finiteIteratorWF) (InvImage FiniteIteratorWF.lt finiteIteratorWF)
-
-theorem descending_step {α β : Type u} [Monad m] [Iterator α m β] {it₁ it₁' : α}
-    (h : (IterStep.successor <$> Iteration.step it₁).prop (some it₁')) :
-    (finiteIteratorWF it₁').lt (finiteIteratorWF it₁) := by
-  simp only [Iteration.prop_map, Iteration.step] at h
-  obtain ⟨step, h, h'⟩ := h
-  split at h' <;> cases h
-  · exact Or.inl ⟨_, h'⟩
-  · exact Or.inr h'
-
-theorem successor_skip {α β : Type u} {m : Type u → Type u} [Monad m] [Iterator α m β] {it₁ it₂ : α} :
-    (IterStep.successor <$> pure (f := Iteration m) (IterStep.skip it₁ True.intro : RawStep α β)).prop (some it₂) ↔
-      it₂ = it₁ := by
-  simp [Iteration.prop_map, Pure.pure, Iteration.pure, IterStep.successor]
-
-theorem successor_yield {α β : Type u} {m : Type u → Type u} [Monad m] [Iterator α m β] {it₁ it₂ : α} {b} :
-    (IterStep.successor <$> pure (f := Iteration m) (IterStep.yield it₁ b True.intro : RawStep α β)).prop (some it₂) ↔
-      it₂ = it₁ := by
-  simp [Iteration.prop_map, Pure.pure, Iteration.pure, IterStep.successor]
-
-theorem successor_done {α β : Type u} {m : Type u → Type u} [Monad m] [Iterator α m β] {it: α} :
-    (IterStep.successor <$> pure (f := Iteration m) (IterStep.done True.intro : RawStep α β)).prop (some it) ↔
-      False := by
-  simp [Iteration.prop_map, Pure.pure, Iteration.pure, IterStep.successor]
 
 theorem descending_flatMapStepNone {α β α' β' : Type u} {m : Type u → Type u} {f : β → α'}
     [Monad m] [Iterator α m β] [Iterator α' m β']
